parser

compiler/scheme/scheme_parsingScript.sml
@@ -9,27 +9,95 @@ open scheme_astTheory;
 val _ = new_theory "scheme_parsing";
 
 
+val _ = monadsyntax.declare_monad("sum", {
+  unit = “INR”,
+  bind = “λ s f . case s of
+    | INL l => INL l
+    | INR r => f r”,
+  ignorebind = NONE,
+  fail = NONE,
+  guard = NONE,
+  choice = SOME “λ x y . case x of
+    | INL l => y
+    | INR r => INR r”
+});
+
+val _ = monadsyntax.enable_monadsyntax();
+val _ = monadsyntax.enable_monad "sum";
+
+Definition mapM_def:
+  mapM f [] = return [] ∧
+  mapM f (x::xs) = do
+      e <- f x;
+      es <- mapM f xs;
+      return (e::es)
+    od
+End
+
 (* lexing *)
 
 Datatype:
   token = OPEN | CLOSE | DOT | NUM num | QUOTE num
+    | PLUS | MINUS | TIMES | BOOL bool | WORD string
 End
 
+Definition delimits_next_def:
+  delimits_next [] = T ∧
+  delimits_next (c::cs) = MEM c " \t\n()#;"
+End
+
+Definition read_bool_def:
+  read_bool (#"#"::c::cs) = (
+    if delimits_next cs then
+      if MEM c "tT" then SOME (T, cs) else
+      if MEM c "fF" then SOME (F, cs) else
+        NONE
+    else NONE) ∧
+  read_bool (_::cs) = NONE
+End
+
+Theorem read_bool_length:
+  ∀ b c cs ys .
+    read_bool (c::cs) = SOME (b,ys) ⇒
+    LENGTH ys ≤ LENGTH cs
+Proof
+  Cases_on ‘cs’ >> rw [read_bool_def, delimits_next_def]
+QED
+
 Definition read_num_def:
-  read_num l h f x acc [] = (acc,[]) ∧
   read_num l h f x acc (c::cs) =
     if ORD l ≤ ORD c ∧ ORD c ≤ ORD h then
-      read_num l h f x (f * acc + (ORD c - x)) cs
-    else (acc,c::cs)
+      let newacc = (f * acc + (ORD c - x)) in
+        if delimits_next cs then SOME (newacc, cs) else
+          read_num l h f x newacc cs
+    else NONE
 End
 
 Theorem read_num_length:
-  ∀l h xs n ys f acc x.
-    read_num l h f x acc xs = (n,ys) ⇒
-    LENGTH ys ≤ LENGTH xs ∧ (xs ≠ ys ⇒ LENGTH ys < LENGTH xs)
+  ∀l h c cs n ys f acc x.
+    read_num l h f x acc (c::cs) = SOME (n,ys) ⇒
+    LENGTH ys ≤ LENGTH cs
 Proof
-  Induct_on ‘xs’ \\ rw [read_num_def]
-  \\ TRY pairarg_tac \\ fs [] \\ rw [] \\ res_tac \\ fs []
+  Induct_on ‘cs’ >> rw [Once read_num_def, delimits_next_def] >> rw[]
+  >> last_assum $ drule >> rw[]
+QED
+
+Definition read_word_def:
+  read_word (c::cs) = if delimits_next cs then SOME ([c], cs) else
+    case read_word cs of
+    | NONE => NONE
+    | SOME (ws, cs') => SOME (c::ws, cs')
+End
+
+Theorem read_word_length:
+  ∀ w c cs ys .
+    read_word (c::cs) = SOME (w,ys) ⇒
+    LENGTH ys ≤ LENGTH cs
+Proof
+  Induct_on ‘cs’ >> rw [Once read_word_def, delimits_next_def] >> gvs[]
+  >> Cases_on ‘read_word (STRING h cs)’ >> gvs[]
+  >> PairCases_on ‘x’ >> gvs[]
+  >> last_assum $ drule >> rw[]
 QED
 
 Definition end_line_def:
@@ -44,65 +112,195 @@ Proof
 QED
 
 Definition lex_def:
-  lex q [] acc = acc ∧
-  lex q (c::cs) acc =
-      if MEM c " \t\n" then lex NUM cs acc else
-      if c = #"#" then lex NUM (end_line cs) acc else
-      if c = #"." then lex NUM cs (DOT::acc) else
-      if c = #"(" then lex NUM cs (OPEN::acc) else
-      if c = #")" then lex NUM cs (CLOSE::acc) else
-      if c = #"'" then lex QUOTE cs acc else
-        let (n,rest) = read_num #"0" #"9" 10 (ORD #"0") 0 (c::cs) in
-          if rest ≠ c::cs then lex NUM rest (q n::acc) else
-            let (n,rest) = read_num #"*" #"z" 256 0 0 (c::cs) in
-              if rest ≠ c::cs then lex NUM rest (q n::acc) else
-                lex NUM cs acc
+  lex [] acc = INR acc ∧
+  lex (c::cs) acc =
+      if MEM c " \t\n" then lex cs acc else
+      if c = #";" then lex (end_line cs) acc else
+      if c = #"." then lex cs (DOT::acc) else
+      if c = #"(" then lex cs (OPEN::acc) else
+      if c = #")" then lex cs (CLOSE::acc) else
+      if c = #"+" then lex cs (PLUS::acc) else
+      if c = #"-" then lex cs (MINUS::acc) else
+      if c = #"*" then lex cs (TIMES::acc) else
+      (*if c = #"'" then lex QUOTE cs acc else*)
+        case read_bool (c::cs) of
+        | SOME (b, rest) => lex rest (BOOL b::acc)
+        | NONE => case read_num #"0" #"9" 10 (ORD #"0") 0 (c::cs) of
+          | SOME (n, rest) => lex rest (NUM n::acc)
+          | NONE => case read_word (c::cs) of
+            | SOME (w, rest) => lex rest (WORD w::acc)
+            | NONE => INL ("Failed to parse at character " ++ [c])
 Termination
-  WF_REL_TAC ‘measure (LENGTH o FST o SND)’ \\ rw []
-  \\ imp_res_tac (GSYM read_num_length) \\ fs [end_line_length]
+  WF_REL_TAC ‘measure (LENGTH o FST)’ >> rw []
+  >- (dxrule read_bool_length >> rw[])
+  >- (dxrule read_word_length >> rw[])
+  >- (dxrule read_num_length >> rw[])
+  >> simp [end_line_length]
 End
 
 Definition lexer_def:
-  lexer input = lex NUM input []
+  lexer input = lex input []
 End
 
 
 (* parsing *)
 
-Definition quote_def:
+(*Definition quote_def:
   quote n = list [Num (name "'"); Num n]
-End
+End*)
 
 Definition parse_def:
-  parse [] x s = x ∧
-  parse (CLOSE :: rest) x s = parse rest (Num 0) (x::s) ∧
+  parse [] x [] = INR x ∧
+  parse [] x s = INL "Too many close brackets" ∧
+  parse (CLOSE :: rest) x s = parse rest Nil (x::s) ∧
   parse (OPEN :: rest) x s =
-    (case s of [] => parse rest x s
+    (case s of [] => INL "Too many open brackets"
      | (y::ys) => parse rest (Pair x y) ys) ∧
-  parse (NUM n :: rest) x s = parse rest (Pair (Num n) x) s ∧
-  parse (QUOTE n :: rest) x s = parse rest (Pair (quote n) x) s ∧
+  parse (NUM n :: rest) x s = parse rest (Pair (Num &n) x) s ∧
+  parse (BOOL b :: rest) x s = parse rest (Pair (Bool b) x) s ∧
+  parse (WORD w :: rest) x s = parse rest (Pair (Word w) x) s ∧
+  parse (PLUS :: rest) x s = parse rest (Pair (Word "+") x) s ∧
+  parse (MINUS :: rest) x s = parse rest (Pair (Word "-") x) s ∧
+  parse (TIMES :: rest) x s = parse rest (Pair (Word "*") x) s ∧
+  (*parse (QUOTE n :: rest) x s = parse rest (Pair (quote n) x) s ∧*)
   parse (DOT :: rest) x s = parse rest (head x) s
 End
 
 (*
-EVAL “head (parse (lexer "(print hi)") (Num 0) [])”
+EVAL “case lexer "(print hi)" of
+| INL x => INL x
+| INR y => case parse y Nil [] of
+  | INL x => INL x
+  | INR y => INR (head y)”
 *)
 
 
 (* conversion to AST *)
 
+Definition pair_to_list_def:
+  pair_to_list Nil = SOME [] ∧
+  pair_to_list (Pair x y) = (case pair_to_list y of
+  | NONE => NONE
+  | SOME xs => SOME (x::xs)) ∧
+  pair_to_list v = NONE
+End
+
+Theorem pair_to_list_size:
+  ∀ p ls . pair_to_list p = SOME ls ⇒ v_size p = list_size v_size ls
+Proof
+  ho_match_mp_tac pair_to_list_ind
+  >> simp[pair_to_list_def, list_size_def]
+  >> rpt strip_tac
+  >> Cases_on ‘pair_to_list p’ >> gvs[list_size_def]
+QED
+
+Definition cons_formals_def:
+  cons_formals ps Nil = INR (REVERSE ps, NONE) ∧
+  cons_formals ps (Word w) = INR (REVERSE ps, SOME (strlit w)) ∧
+  cons_formals ps (Pair (Word x) y) = cons_formals (strlit x::ps) y ∧
+  cons_formals ps _ = INL "Invalid lambda formals"
+End
+
+Definition cons_ast_def:
+  cons_ast (Num n) = INR (Val (SNum n)) ∧
+  cons_ast (Bool b) = INR (Val (SBool b)) ∧
+  cons_ast (Word w) = (
+    if w = "+" then INR (Val (Prim SAdd)) else
+    if w = "-" then INR (Val (Prim SMinus)) else
+    if w = "*" then INR (Val (Prim SMul)) else
+    if w = "eqv?" then INR (Val (Prim SEqv)) else
+    if w = "callcc" then INR (Val (Prim CallCC)) else
+      INR (Ident (strlit w))) ∧
+  cons_ast Nil = INL "Empty S expression" ∧
+  cons_ast (Pair x y) = (case pair_to_list y of
+  | NONE => INL "Invalid S expression"
+  | SOME ys => (case x of
+    | Word "if" => (case ys of
+      | [c;t;f] => do
+          ce <- cons_ast c;
+          te <- cons_ast t;
+          fe <- cons_ast f;
+          return (Cond ce te fe)
+        od
+      | _ => INL "Wrong number of expressions in if statement")
+    | Word "begin" => (case ys of
+      | [] => INL "Wrong number of expressions to begin"
+      | y'::ys' => do
+          e <- cons_ast y';
+          es <- cons_ast_list ys';
+          return (Begin e es)
+        od)
+    | Word "lambda" => (case ys of
+      | [xs;y'] => do
+          (ps,lp) <- cons_formals [] xs;
+          e <- cons_ast y';
+          return (Lambda ps lp e)
+        od
+      | _ => INL "Wrong number of expressions in lambda statement")
+    | Word "letrec" => (case ys of
+      | [xs;y'] => (case pair_to_list xs of
+        | NONE => INL "Invalid S expression"
+        | SOME xs' => do
+            bs <- cons_ast_bindings xs';
+            e <- cons_ast y';
+            return (Letrec bs e)
+          od)
+      | _ => INL "Wrong number of expressions in letrec statement")
+    | Word "set!" => (case ys of
+      | [Word w;y'] => do
+          e <- cons_ast y';
+          return (Set (strlit w) e)
+        od
+      | _ => INL "Invalid set expression")
+    | fn => do
+        e <- cons_ast fn;
+        es <- cons_ast_list ys;
+        return (Apply e es)
+      od)) ∧
+
+  cons_ast_list [] = INR [] ∧
+  cons_ast_list (x::xs) = (do
+      e <- cons_ast x;
+      es <- cons_ast_list xs;
+      return (e::es)
+    od) ∧
+
+  cons_ast_bindings [] = INR [] ∧
+  cons_ast_bindings (x::xs) = (case pair_to_list x of
+  | NONE => INL "Invalid S expression"
+  | SOME ys => (case ys of
+    | [Word w;b] => do
+        e <- cons_ast b;
+        es <- cons_ast_bindings xs;
+        return ((strlit w, e)::es)
+      od
+    | _ => INL "Invalid letrec binding"))
+Termination
+  WF_REL_TAC ‘measure $ λ x . case x of
+    | INL v => v_size v
+    | INR (INL vs) => list_size v_size vs
+    | INR (INR vs') => list_size v_size vs'’
+  >> rpt strip_tac
+  >> rpt (
+    dxrule_then (assume_tac o GSYM) pair_to_list_size
+    >> gvs[list_size_def]
+  )
+End
+
 Definition parse_to_ast_def:
-  parse_to_ast s =
-    let e = head (parse (lexer s) (Num 0) []) in
-      if e = Pair (Name "print") (Pair (Name "hi") (Num 0)) then
-        INR (Print (strlit "hi\n"))
-      else
-        INL ("This version can only parse '(print hi)'.")
+  parse_to_ast s = do
+      lxs <- lexer s;
+      e <- parse lxs Nil [];
+      cons_ast (head e)
+    od
 End
 
 (*
-EVAL “parse_to_ast "(print hi)"”
-EVAL “parse_to_ast "(print hello)"”
+EVAL “cons_ast (Pair (Word "print") (Pair (Word "hi") Nil))”
+EVAL “do e <- do es' <- mapM cons_ast [Word "t"; Word "h"]; return (Apply (Val (SNum 0)) es') od; es <- mapM cons_ast [Pair (Word "+") Nil; Word "-"]; return (Apply e es) od”
+EVAL “parse_to_ast "((if #t + * ) 2 3)"”
+EVAL “parse_to_ast "(lambda (x y . l) 2)"”
+EVAL “parse_to_ast "(letrec ((x 3) (y x)) 2)"”
 *)
 
 val _ = export_theory();
