compiler/scheme/scheme_to_cakeScript.sml
@@ -457,6 +457,10 @@ val _ = export_theory();
       )
     ))] (Apply (Ident $ strlit "fac") [Val $ SNum 6])
   )]”
+
+  open scheme_parsingTheory;
+  EVAL “SND $ evaluate <| clock := 999; refs := [] |> myEnv [scheme_program_to_cake $ OUTR $ parse_to_ast
+    "(letrec ((fac (lambda (x) (letrec ((st 0) (acc 1)) (begin (callcc (lambda (k) (set! st k))) (if (eqv? x 0) acc (st (begin (set! acc ( * acc x)) (set! x (- x 1)))))))))) (fac 6))"]”
   EVAL “scheme_program_to_cake (Cond (Val $ SBool F) (Val $ SNum 420) (Val $ SNum 69))”
   EVAL “scheme_program_to_cake (Apply (Val $ Prim SMul) [Val $ SNum 2; Val $ SNum 3])”
   EVAL “scheme_program_to_cake (Apply (Lambda [] (SOME $ strlit "x") (Ident $ strlit "x")) [Val $ SNum 5])”
